theories/Trace.v
@@ -1,0 +1,13 @@
+From HTTP Require Export
+     Tcp.
+
+Variant traceT :=
+  Trace__In  : packetT id -> traceT
+| Trace__Out : packetT id -> traceT.
+
+Instance Serialize__traceT : Serialize traceT :=
+  fun t =>
+    match t with
+    | Trace__In  p => [Atom "In "; to_sexp p]
+    | Trace__Out p => [Atom "Out"; to_sexp p]
+    end%sexp.
